src/coq/optimisations/StaticAnalysis/const_prop.v
@@ -2,7 +2,6 @@ Require Import ZArith List String Omega.
 Require Import Vellvm.Ollvm_ast Vellvm.Classes Vellvm.Util Vellvm.CFGProp Vellvm.CFG.
 Require Import Vellvm.optimisations.paco_util.
 Require Import Vellvm.optimisations.step_trace.
-Require Import Vellvm.optimisations.EqNat.
 Require Import Vellvm.optimisations.SSA_semantics.
 
 Require Import Vellvm.DecidableEquality.
