src/coq/optimisations/eq_dec.v
@@ -1,0 +1,516 @@
+Require Import ZArith.ZArith List.
+Require Import String Omega.
+Require Import Vellvm.Ollvm_ast Vellvm.Classes Vellvm.Util.
+Require Import Vellvm.optimisations.vellvm_tactics.
+Require Import Vellvm.optimisations.local_cfg.
+Require Import Vellvm.optimisations.map_spec.
+
+Require Import Equalities.
+Require Import OrderedType.
+Require Import OrderedTypeEx.
+Require Import Compare_dec.
+Require Import Bool.
+Require Import Coq.MSets.MSetGenTree.
+Import ListNotations.
+Set Implicit Arguments.
+
+
+Print OrderedType. 
+Instance eq_dec_int : eq_dec int := Z_eq_dec.
+Require Import Ascii.
+
+
+
+Module AsciiOrd <: OrderedType.
+  Definition t := ascii.
+  Definition eq := @eq t.
+    Scheme Equality for ascii.
+  Definition lt (a b:ascii) := N.lt (N_of_ascii a) (N_of_ascii b).
+  Definition eq_refl := @eq_refl t.
+  Definition eq_sym := @eq_sym t.
+  Definition eq_trans := @eq_trans t.
+ 
+
+  Ltac destr_simpl x y := destruct x eqn:?; simpl in *; inv y.
+
+    Lemma eq_correct : forall a b, eq a b <-> ascii_beq a b = true.
+  Proof. split; intros. 
+         unfold eq in *. subst. destruct b; simpl in *. assert (forall a, bool_beq a a = true). intros. destruct a; simpl in *; eauto. repeat rewrite H. simpl. eauto.
+
+destruct a, b. simpl in *. 
+destr_simpl (bool_beq b0 b) H; destr_simpl (bool_beq b1 b8) H; destr_simpl (bool_beq b2 b9) H; destr_simpl (bool_beq b3 b10) H; destr_simpl (bool_beq b4 b11) H; destr_simpl (bool_beq b5 b12) H; destr_simpl (bool_beq b6 b13) H.
+
+assert (forall a c, bool_beq a c = true -> a = c).  intros. destruct a, c; eauto.
+eapply H0 in Heqb15; eapply H0 in Heqb0; eapply H0 in Heqb1; eapply H0 in Heqb2; eapply H0 in Heqb3; eapply H0 in Heqb4; eapply H0 in Heqb5; eapply H0 in H; subst; eapply eq_refl. Qed.
+
+Lemma beq_refl : forall a, ascii_beq a a = true.
+  Proof. intros. eapply eq_correct. eapply eq_refl. Qed.
+
+
+  
+  Lemma lt_trans : forall a b c:t, lt a b -> lt b c -> lt a c.
+  Proof.
+    intros a b c.
+    unfold lt.
+    apply N.lt_trans.
+  Qed.
+
+  Lemma lt_not_eq : forall a b:t, lt a b -> ~eq a b.
+  Proof.
+    intros a b H.
+    unfold eq. unfold not. intros He. rewrite He in H.
+    eapply N.lt_neq. unfold lt in H. apply H. reflexivity.
+  Qed.
+  
+
+    Lemma N_of_ascii_inj : forall x y, N_of_ascii x = N_of_ascii y -> x = y.
+  Proof.
+    intros x y H.
+    rewrite <- ascii_N_embedding.
+    rewrite <- (@ascii_N_embedding x).
+    rewrite H. reflexivity.
+  Defined.
+
+    Program Definition compare (x y: t) : Compare lt eq x y :=
+    match N_as_OT.compare (N_of_ascii x) (N_of_ascii y) with
+    | LT p => _
+    | EQ p => _
+    | GT p => _
+    end.
+  Next Obligation.
+    apply LT. unfold lt. auto.
+  Defined.
+  Next Obligation.
+    apply EQ. unfold eq. apply N_of_ascii_inj. auto.
+  Defined.
+  Next Obligation.
+    apply GT. unfold lt. auto.
+  Defined.
+  Definition eq_dec := ascii_dec.
+
+End AsciiOrd.
+Module AsciiOrdFacts := OrderedTypeFacts(AsciiOrd).
+
+Module StringOrd <: OrderedType.
+  Definition t := string.
+    Definition eq := @eq t.
+  Definition eq_refl := @eq_refl t.
+  Definition eq_sym := @eq_sym t.
+  Definition eq_trans := @eq_trans t.
+    Fixpoint lt (s1 s2:string) : Prop :=
+    match s1, s2 with
+    | EmptyString, EmptyString => False
+    | EmptyString, String _ _ => True
+    | String a s1', String b s2' =>
+      match AsciiOrd.compare a b with
+      | LT _ => True
+      | EQ _ => lt s1' s2'
+      | GT _ => False
+      end
+    | String _ _, EmptyString => False
+    end.
+
+  Lemma lt_trans : forall a b c : t, lt a b -> lt b c -> lt a c.
+  Proof.
+    induction a.
+    - destruct b; destruct c; simpl; intros; try tauto.
+    - destruct b; destruct c; simpl; intros; try tauto.
+      destruct (AsciiOrd.compare a a1); try tauto.
+      + destruct (AsciiOrd.compare a1 a2); try tauto.
+        * AsciiOrdFacts.elim_comp; auto.
+        * AsciiOrdFacts.elim_comp; auto.
+      + destruct (AsciiOrd.compare a1 a2); try tauto.
+        * AsciiOrdFacts.elim_comp; auto.
+        * AsciiOrdFacts.elim_comp; auto.
+          eapply IHa; eauto.
+  Qed.          
+      
+  Lemma lt_not_eq : forall a b:t, lt a b -> ~eq a b.
+  Proof.
+    induction a; intros b H He; unfold eq in He; subst.
+    - unfold lt in H. destruct H.
+    - simpl in H.
+      destruct (AsciiOrd.compare a a); auto.
+      apply AsciiOrd.lt_not_eq in l. apply l. AsciiOrdFacts.order.
+      apply IHa in H. apply H. unfold eq. reflexivity.
+  Qed.
+
+
+    Program Fixpoint compare (s1 s2 : t) : Compare lt eq s1 s2 :=
+    match s1, s2 with
+    | EmptyString, EmptyString => _
+    | EmptyString, String b s2' => _
+    | String a s1', String b s2' =>
+      match AsciiOrd.compare a b with
+      | LT _ => _
+      | EQ _ => match compare s1' s2' with
+               | LT _ => _
+               | EQ _ => _
+               | GT _ => _
+               end
+      | GT _ => _ 
+      end
+    | String a s1', EmptyString => _
+    end.
+  Next Obligation.
+    apply EQ. unfold eq. reflexivity.
+  Defined.
+  Next Obligation.
+    apply LT. simpl. auto.
+  Defined.
+  Next Obligation.
+    apply LT. simpl. rewrite <- Heq_anonymous. auto.
+  Defined.
+  Next Obligation.
+    apply LT. simpl. rewrite <- Heq_anonymous0. auto.
+  Defined.
+  Next Obligation.
+    apply EQ. simpl. unfold AsciiOrd.eq in wildcard'0. subst. unfold eq in e. subst. reflexivity.
+  Defined.
+  Next Obligation.
+    apply GT. simpl. unfold AsciiOrd.eq in wildcard'0. subst.
+    rewrite <- Heq_anonymous0. auto.
+  Defined.
+  Next Obligation.
+    apply GT. simpl. AsciiOrdFacts.elim_comp_lt b a. auto.
+  Defined.
+  Next Obligation.
+    apply GT. simpl. auto.
+  Defined.
+
+  Definition eq_dec := string_dec.
+
+  Fixpoint string_beq (a b: string) :=
+    match a, b with
+    | EmptyString, EmptyString => true
+    | String s1 t1, String s2 t2 => AsciiOrd.ascii_beq s1 s2 && string_beq t1 t2
+    | _, _ => false
+    end.
+
+
+    Lemma beq_refl : forall a, string_beq a a = true.
+    Proof. induction a; eauto. simpl in *. rewrite AsciiOrd.beq_refl. simpl in *. eauto. Qed.
+
+    
+    Lemma beq_correct : forall a b, string_beq a b = true <-> a = b.
+  Proof. induction a, b; split; intros; eauto.
+         +inversion H.
+         +inversion H.
+         +inversion H.
+         +inversion H.
+         +inversion H. simpl in *.
+          destruct ( AsciiOrd.ascii_beq) eqn:?.
+         -simpl in *. eapply IHa in H. subst. eapply AsciiOrd.eq_correct in Heqb0. inversion Heqb0. subst. eauto.
+         -simpl in *. inversion H.
+         +rewrite H.  simpl. rewrite AsciiOrd.beq_refl. simpl in *. rewrite beq_refl. eauto. Qed.
+
+
+  
+End StringOrd.
+Module StringOrdFacts := OrderedTypeFacts(StringOrd).
+
+
+
+
+
+
+
+Module RawIDOrd <: OrderedType.
+  Definition t := raw_id.
+
+  Definition eq := @eq t.
+  Definition eq_refl := @eq_refl t.
+  Definition eq_sym := @eq_sym t.
+  Definition eq_trans := @eq_trans t.
+
+  
+  (* Anon < Name < Raw *)
+  Definition lt (x:t) (y:t) : Prop :=
+    match x,y with
+    | Anon n1, Anon n2 => (n1 < n2)%Z
+    | Name s1, Name s2 => StringOrd.lt s1 s2
+    | Raw n1, Raw n2 => (n1 < n2)%Z
+    | Anon _, _ => True
+    | Name _, Raw _ => True
+    | _, _ => False 
+    end.
+
+  Lemma lt_trans : forall a b c : t, lt a b -> lt b c -> lt a c.
+  Proof.
+    destruct a; destruct b; destruct c; simpl; intros H1 H2; intuition.
+    - eapply StringOrd.lt_trans; eauto.
+  Qed.
+
+  Lemma lt_not_eq : forall a b:t, lt a b -> ~eq a b.
+  Proof.
+    destruct a; destruct b; simpl; intros H He; inversion He; subst.
+    - apply StringOrd.lt_not_eq in H. apply H. unfold StringOrd.eq. reflexivity.
+    - apply Z_as_OT.lt_not_eq in H. tauto.
+    - apply Z_as_OT.lt_not_eq in H. tauto.
+  Qed.
+
+
+         
+  Program Definition compare (x:t) (y:t) : Compare lt eq x y :=
+    match x,y with
+    | Anon n1, Anon n2 =>
+      match Z_as_OT.compare n1 n2 with
+      | LT _ => LT _
+      | EQ _ => EQ _
+      | GT _ => GT _
+      end
+    | Anon _, Name _ => LT _
+    | Anon _, Raw _ => LT _
+    | Name _, Anon _ => GT _
+    | Name s1, Name s2 =>
+      match StringOrd.compare s1 s2 with
+      | LT _ => LT _
+      | EQ _ => EQ _
+      | GT _ => GT _
+      end
+    | Name _, Raw _ => LT _
+    | Raw _, Anon _ => GT _
+    | Raw _, Name _ => GT _
+    | Raw n1, Raw n2 =>
+      match Z_as_OT.compare n1 n2 with
+      | LT _ => LT _
+      | EQ _ => EQ _
+      | GT _ => GT _
+      end
+    end.
+  Next Obligation.
+    unfold Z_as_OT.eq in wildcard'. subst. unfold eq. reflexivity.
+  Defined.
+  Next Obligation.
+    unfold StringOrd.eq in wildcard'. subst. unfold eq. reflexivity.
+  Defined.
+  Next Obligation.
+    unfold Z_as_OT.eq in wildcard'. subst. unfold eq. reflexivity.
+  Defined.
+
+
+  Definition beq (t1 t2: raw_id) :=
+    match t1, t2 with
+    | Anon n1, Anon n2 => Z.eqb n1 n2
+    | Name s1, Name s2 => StringOrd.string_beq s1 s2
+    | Raw n1, Raw n2 => Z.eqb n1 n2
+    | _, _ => false
+    end.
+
+  Lemma beq_refl : forall a, beq a a = true.
+  Proof. unfold beq; destruct a. eapply StringOrd.beq_correct. eauto.
+apply Z.eqb_refl. apply Z.eqb_refl. Qed.
+Hint Resolve beq_refl.
+         
+  Lemma beq_correct : forall a b, beq a b = true <-> eq a b.
+  Proof. induction a, b; split; intros; try inv H.
+         +eapply StringOrd.beq_correct in H1. subst. apply eq_refl.
+         +eapply Z.eqb_eq in H1. subst. eapply eq_refl.
+         +eapply Z.eqb_eq in H1. subst. eapply eq_refl. Qed.
+
+  Lemma lt_false :  forall lbk1 lbk0, lt lbk1 lbk0 ->  lt lbk0 lbk1 -> False.
+  Proof. intros. destruct lbk1, lbk0; simpl in *; try inv H; try inv H0.
+         +eapply StringOrd.lt_trans in H; eauto. eapply StringOrd.lt_not_eq in H. contradiction H. unfold StringOrd.eq. eauto.
+         +eapply Z.lt_asymm in H. tauto.
+         +eapply Z.lt_asymm in H. tauto. Qed.
+
+
+  Definition eq_dec : forall (x y : t), {x = y} + {x <> y}.
+    decide equality.
+    - apply string_dec.
+    - apply eq_dec_int.
+    - apply eq_dec_int.
+  Defined.
+
+End RawIDOrd.  
+
+Instance eq_dec_raw_id : eq_dec raw_id := RawIDOrd.eq_dec.
+
+
+
+
+Module InstrIDOrd <: OrderedType.
+  Definition t := instr_id.
+
+  Definition eq := @eq t.
+  Definition eq_refl := @eq_refl t.
+  Definition eq_sym := @eq_sym t.
+  Definition eq_trans := @eq_trans t.
+
+  
+  Print instr_id.
+  Definition beq (t1 t2:t) :=
+    match t1, t2 with
+    | IId i1, IId i2 => RawIDOrd.beq i1 i2
+    | IVoid i1, IVoid i2 => Z.eqb i1 i2
+    | _, _ => false
+    end.
+
+
+  Lemma beq_refl : forall t1, beq t1 t1 = true.
+  Proof. destruct t1; simpl in *. eapply RawIDOrd.beq_refl. eapply Z.eqb_refl. Qed.
+  Hint Resolve beq_refl.
+  
+  Lemma beq_correct : forall t1 t2,  beq t1 t2 = true <-> eq t1 t2.
+  Proof. destruct t1, t2; split; intros; try inv H; eauto.
+         + eapply  RawIDOrd.beq_correct in H1. unfold RawIDOrd.eq in *. subst. eapply eq_refl.
+         + eapply Z.eqb_eq in H1. subst. unfold eq. eauto. Qed.
+  
+(*IVoid < IId*)  
+  Definition lt (x:t) (y:t) : Prop :=
+    match x,y with
+    | IVoid n1, IVoid n2 => (n1 < n2)%Z
+    | IId s1, IId s2 => RawIDOrd.lt s1 s2
+    | IVoid _, IId _ => False
+    | IId _, IVoid _ => True
+    end.
+  
+    Lemma lt_trans : forall a b c : t, lt a b -> lt b c -> lt a c.
+  Proof.
+    destruct a; destruct b; destruct c; simpl; intros H1 H2; intuition.
+    eapply RawIDOrd.lt_trans; eauto.
+  Qed.
+  
+  Lemma lt_not_eq : forall a b:t, lt a b -> ~eq a b.
+  Proof.
+    destruct a; destruct b; simpl; intros H He; inversion He; subst.
+    - apply RawIDOrd.lt_not_eq in H. unfold not in H. unfold RawIDOrd.eq in *. unfold eq in He. eapply H. eauto.
+    - apply Z_as_OT.lt_not_eq in H. tauto.
+  Qed.
+
+  Program Definition compare (x:t) (y:t) : Compare lt eq x y :=
+    match x, y with
+    | IId n1, IId n2 => match RawIDOrd.compare n1 n2 with
+                        | LT _ => LT _
+                        | EQ _ => EQ _
+                        | GT _ => GT _                        
+                        end
+                          
+    | IId _, IVoid _ => LT _
+    | IVoid n1, IVoid n2 => match Z_as_OT.compare n1 n2 with
+                             | LT _ => LT _
+                             | EQ _ => EQ _
+                             | GT _ => GT _
+                             end
+    | IVoid _, IId _ => GT _
+    end.
+  Next Obligation. unfold RawIDOrd.eq in *. subst. unfold eq. eauto. Defined.
+  Next Obligation. unfold Z_as_OT.eq in *. subst. unfold eq. eauto. Defined.
+
+
+
+  Definition eq_dec : forall (x y : t), {x = y} + {x <> y}.
+    decide equality.
+    -eapply  eq_dec_raw_id.
+    -eapply eq_dec_int.
+     Defined.
+
+
+  
+End InstrIDOrd.
+Instance eq_dec_instr_id : eq_dec instr_id := InstrIDOrd.eq_dec.
+
+
+
+
+
+
+Module Local_PCOrd <: OrderedType.
+    Definition t := local_pc.
+  
+  Definition eq := @eq t.
+  Definition eq_refl := @eq_refl t.
+  Definition eq_sym := @eq_sym t.
+  Definition eq_trans := @eq_trans t.
+
+  Definition beq (t1 t2: local_pc) : bool := RawIDOrd.beq (lbk t1) (lbk t2) && InstrIDOrd.beq (lpt t1) (lpt t2).
+
+  Lemma beq_refl : forall t1, beq t1 t1 = true.
+  Proof. unfold beq; destruct t1; simpl in *. rewrite RawIDOrd.beq_refl. simpl. rewrite InstrIDOrd.beq_refl. auto. Qed.
+
+
+  Lemma beq_correct : forall t1 t2, beq t1 t2 = true <-> eq t1 t2.
+  Proof. induction t1, t2; unfold beq; simpl in *; split; intros; unfold eq.
+         +destruct ( RawIDOrd.beq lbk lbk0) eqn:?; destruct (InstrIDOrd.beq lpt lpt0) eqn:?; simpl in *.
+          *eapply RawIDOrd.beq_correct in Heqb. unfold RawIDOrd.eq in *. subst. eapply InstrIDOrd.beq_correct in Heqb0. unfold InstrIDOrd.eq in *. subst. eauto.
+          *inversion H.
+          *inversion H.
+          *inversion H.
+         +unfold eq in *. inversion H. subst. rewrite RawIDOrd.beq_refl. rewrite InstrIDOrd.beq_refl. simpl in *. eauto. Qed.
+
+
+    Definition lt (x:t) (y:t) : Prop :=
+      match RawIDOrd.beq (lbk x) (lbk y) with
+      | true => InstrIDOrd.lt (lpt x) (lpt y)
+      | false => RawIDOrd.lt (lbk x) (lbk y)
+      end.
+
+
+
+  Lemma lt_trans : forall a b c : t, lt a b -> lt b c -> lt a c.
+  Proof.
+    destruct a; destruct b; destruct c. simpl in *. unfold lt. simpl in *. intros.
+    destruct (RawIDOrd.beq lbk lbk0) eqn:?, (RawIDOrd.beq lbk0 lbk1) eqn:?, (RawIDOrd.beq lbk lbk1) eqn:?.
+    +simpl in *. eapply RawIDOrd.beq_correct in Heqb. unfold RawIDOrd.eq in *. subst. eapply RawIDOrd.beq_correct in Heqb0. unfold RawIDOrd.eq in *. subst. eapply InstrIDOrd.lt_trans; eauto.
+    +eapply RawIDOrd.beq_correct in Heqb. eapply RawIDOrd.beq_correct in Heqb0. unfold RawIDOrd.eq in *. subst. rewrite RawIDOrd.beq_refl in Heqb1. inversion Heqb1.
+    +eapply RawIDOrd.beq_correct in Heqb. eapply RawIDOrd.beq_correct in Heqb1. unfold RawIDOrd.eq in *. subst. rewrite RawIDOrd.beq_refl in Heqb0. inversion Heqb0.
+    +eapply RawIDOrd.beq_correct in Heqb. unfold RawIDOrd.eq in *. subst. eauto.
+    +eapply RawIDOrd.beq_correct in Heqb0. eapply RawIDOrd.beq_correct in Heqb1. unfold RawIDOrd.eq in *. subst. rewrite RawIDOrd.beq_refl in Heqb. inversion Heqb.
+    +eapply RawIDOrd.beq_correct in Heqb0. unfold RawIDOrd.eq in *. subst. eauto.
+    +eapply RawIDOrd.beq_correct in Heqb1. unfold RawIDOrd.eq in *. subst. unfold  InstrIDOrd.lt. simpl in *.
+     eapply RawIDOrd.lt_false in H; eauto. inversion H.
+    +eapply RawIDOrd.lt_trans; eauto. Qed.
+
+  Lemma lt_not_eq : forall a b:t, lt a b -> ~eq a b.
+  Proof. intros. destruct a, b. simpl in *. unfold lt in *. simpl in *. unfold eq. simpl in *. unfold not. intros. inversion H0. subst. rewrite RawIDOrd.beq_refl in H. eapply InstrIDOrd.lt_not_eq in H. unfold InstrIDOrd.eq in *. tauto. Qed.
+
+
+
+    Program Definition compare (x:t) (y:t) : Compare lt eq x y :=
+      match RawIDOrd.compare (lbk x) (lbk y) with
+      | LT _ => LT _
+      | EQ _ => match InstrIDOrd.compare (lpt x) (lpt y) with
+                | LT _ => LT _
+                | EQ _ => EQ _
+                | GT _ => GT _           
+                end
+      | GT _ => GT _
+      end.
+    Next Obligation.
+destruct x, y. simpl in *. simpl. unfold lt. simpl in *.
+destruct (RawIDOrd.beq lbk lbk0) eqn:?; eauto. generalize wildcard'. intros. eapply RawIDOrd.lt_not_eq in wildcard'0.  unfold not in wildcard'0.  eapply RawIDOrd.beq_correct in Heqb. tauto.
+    Defined.
+    Next Obligation.
+      destruct x, y. simpl in *. unfold lt. simpl in *. destruct (RawIDOrd.beq lbk lbk0) eqn:?. eapply RawIDOrd.beq_correct in Heqb. unfold RawIDOrd.eq in *. eauto. eauto. assert (RawIDOrd.beq lbk lbk0 = true). eapply RawIDOrd.beq_correct. eauto. rewrite H in Heqb. inversion Heqb.
+      Defined.
+      Next Obligation.
+        destruct x, y. simpl in *. unfold eq. unfold RawIDOrd.eq in *. unfold InstrIDOrd.eq in *. subst. eauto.
+      Defined.
+      Next Obligation.
+        destruct x, y. simpl in *. unfold lt.  simpl in *. destruct (RawIDOrd.beq lbk0 lbk) eqn:?. eapply RawIDOrd.beq_correct in Heqb. unfold RawIDOrd.eq in *. subst. eauto. unfold RawIDOrd.eq in *. subst.
+        assert (RawIDOrd.beq lbk0 lbk0 = true). rewrite RawIDOrd.beq_refl. eauto. rewrite H in Heqb. inversion Heqb.
+      Defined.
+      Next Obligation.
+        destruct y, x. simpl in *. unfold lt. simpl in *. destruct (RawIDOrd.beq lbk lbk0) eqn:?; eauto. eapply RawIDOrd.beq_correct in Heqb. unfold RawIDOrd.eq in *. subst. generalize wildcard'; intros.
+
+
+        eapply RawIDOrd.lt_not_eq in wildcard'0. unfold not in *. unfold RawIDOrd.eq in *. tauto.
+      Defined.
+
+
+  Definition eq_dec : forall (x y : t), {x = y} + {x <> y}.
+    decide equality.
+    -eapply  eq_dec_instr_id.
+    -eapply eq_dec_raw_id.
+     Defined.
+Print compare.
+
+
+      
+End Local_PCOrd.
+
+
+
+Instance eq_dec_local_pc : eq_dec local_pc := Local_PCOrd.eq_dec.
+
+
