src/coq/optimisations/map_spec.v
@@ -1,7 +1,7 @@
 
 Require Import Equivalence EquivDec.
 Require Import Coqlib.
-
+Require Import Equalities.
 Local Unset Elimination Schemes.
 Local Unset Case Analysis Schemes.
 
@@ -101,3 +101,77 @@ Module Type TREE.
     forall (m1: t A) (m2: t B) (i: elt),
     get i (combine f m1 m2) = f (get i m1) (get i m2).
 End TREE.
+
+
+
+
+Module Type TREE1.
+  Parameter elt: Type.
+  Parameter elt_eq: forall (a b: elt), {a = b} + {a <> b}.
+
+  Axiom elt_eq_refl : forall x : elt, eq x x.
+  Axiom elt_eq_sym : forall x y : elt, eq x y -> eq y x.
+  Axiom elt_eq_trans : forall x y z : elt, eq x y -> eq y z -> eq x z.
+  Parameter elt_eqb : elt -> elt -> bool.
+  Parameter elt_eqb_eq : forall x y, elt_eqb x y = true <-> eq x y.
+
+  Parameter val: Type.
+  Parameter val_eq : val -> val -> Prop.
+  Parameter val_eqb : val -> val -> bool.
+  Parameter val_eqb_eq : forall x y, val_eqb x y = true <-> val_eq x y.
+
+
+
+  
+  
+  Parameter t: Type.
+  Parameter empty: t.
+  Parameter get: elt -> t -> option val.
+  Parameter set: elt -> val -> t -> t.
+  Parameter remove: elt -> t -> t.
+
+  Axiom gempty:
+    forall (i: elt), get i (empty) = None.
+  Axiom gss:
+    forall  (i: elt) (x: val) (m: t), get i (set i x m) = Some x.
+  Axiom gso:
+    forall (i j: elt) (x: val) (m: t),
+    i <> j -> get i (set j x m) = get i m.
+  Axiom gsspec:
+    forall (i j: elt) (x: val) (m: t),
+    get i (set j x m) = if elt_eq i j then Some x else get i m.
+  Axiom grs:
+    forall (i: elt) (m: t), get i (remove i m) = None.
+  Axiom gro:
+    forall (i j: elt) (m: t),
+    i <> j -> get i (remove j m) = get i m.
+  Axiom grspec:
+    forall  (i j: elt) (m: t),
+    get i (remove j m) = if elt_eq i j then None else get i m.
+
+
+
+
+  Parameter beq:  t -> t -> bool.
+  
+  Axiom beq_correct:
+    forall  (t1 t2: t),
+    beq t1 t2 = true <->
+    (forall (x: elt),
+     match get x t1, get x t2 with
+     | None, None => True
+     | Some y1, Some y2 => val_eqb y1 y2 = true
+     | _, _ => False
+    end).
+
+
+  Parameter combine:
+    (option val -> option val -> option val) -> t -> t -> t.
+  Axiom gcombine:
+    forall (f: option val -> option val -> option val),
+    f None None = None ->
+    forall (m1: t) (m2: t) (i: elt),
+    get i (combine f m1 m2) = f (get i m1) (get i m2).
+End TREE1.
+
+
